can sum sets

dfy/cnf.dfy
@@ -6,12 +6,23 @@ include "sat.dfy"
 module CNF {
     import opened SAT
 
+function clause_literal_count(c: Clause) : int
+{
+    |c|
+}
+
 function clause_is_tautology(c: Clause) : (out: bool)
     ensures out ==> (
         forall vs: map<Variable,bool> :: true ==> clause_eval(c, vs) == true
     )
 {
     exists l1,l2 :: l1 in c && l2 in c && l1.invert() == l2
+}
+
+
+method cnf_literal_count(cnf: CNF) returns (out: int)
+{
+    out := Util.set_sum(set c | c in cnf :: clause_literal_count(c));
 }
 
 ghost function cnf_equivalent(cnf: CNF, other: CNF) : (eq: bool)
@@ -38,94 +49,20 @@ function cnf_remove_tautologies(cnf: CNF) : (out: CNF)
     set c | c in cnf && !clause_is_tautology(c)
 }
 
-function clause_max_litvar(c: Clause) : (out: ClauseLit)
-    requires |c| > 0
-{
-    var lambda := (l: ClauseLit) => l.number();
-    SAT.NumbersBijection(c, lambda);
-    Util.extract_max_from_set_by_score(c, lambda)
-}
-
-function clause_lt(c1: Clause, c2: Clause) : (out: bool)
-    requires c1 != c2
-{
-    if |c1| < |c2| then
-        true
-    else if |c1| > |c2| then
-        false
-    else
-        var l1 := clause_max_litvar(c1);
-        var l2 := clause_max_litvar(c2);
-        if l1.number() < l2.number() then
-            true
-        else if l1.number() > l2.number() then
-            false
-        else
-            assert l1 == l2;
-            assert c1 - {l1} + {l1} == c1;
-            clause_lt(c1 - {l1}, c2 - {l2})
-}
-
-// lemma WellFormed(s: set<Clause>)
-//     ensures Util.well_ordered(s, (c1,c2) => clause_lt(c1,c2))
-// {
-
-// }
-
-// function max_clause(cnf: CNF) : (out: Clause)
-//     requires |cnf| > 0
-// {
-//     Util.extract_max_from_set_by_order(cnf, clause_lt)
-// }
-
-// function cnf_find_resolution_with_var(cnf: CNF, v: Variable) : (out: set<Clause>)
-//     requires !cnf_has_tautologies(cnf)
-//     // ensures (exists l1, l2, c1, c2 ::
-//     //     v in cnf_vars(cnf) &&
-//     //     c1 in cnf && c2 in cnf && c1 != c2 &&
-//     //     l1 in c1 && NotInverted(v) == l1 &&
-//     //     l2 in c2 && Inverted(v) == l2) <==> |out| == 2
-//     ensures |out| == 0 || |out| == 2
-// {
-//     var where_inverted := set c | c in cnf && Inverted(v) in c;
-//     var where_not_inverted := set c | c in cnf && NotInverted(v) in c;
-//     assert |where_inverted * where_not_inverted| == 0;
-//     if |where_inverted| > 0 && |where_not_inverted| > 0 then
-//         var c1 :| c1 in where_inverted && forall c :: c in where_inverted && c != c1 && c1 > c;
-//         var c2 :| c2 in where_not_inverted;
-//         {c1, c2}
-//     else
-//         {}
-// }
-
-ghost function cnf_resolution_vars(cnf: CNF) : (out: set<Variable>)
-    ensures forall v :: v in out <==> v in cnf_vars(cnf) && cnf_has_resolution_with_var(cnf, v)
-{
-    set v | v in cnf_vars(cnf) && cnf_has_resolution_with_var(cnf, v)
-}
-
 function cnf_has_resolution(cnf: CNF) : (out: bool)
-    ensures out == (exists v :: v in cnf_vars(cnf) && cnf_has_resolution_with_var(cnf, v))
 {
-    exists v :: v in cnf_vars(cnf) && cnf_has_resolution_with_var(cnf, v)
+    exists v, c1, c2 :: v in cnf_vars(cnf) && c1 in cnf && c2 in cnf && cnf_has_resolution_with(cnf, v, c1, c2)
 }
 
-function cnf_has_resolution_with_var(cnf: CNF, v: Variable) : (out: bool)
+function cnf_has_resolution_with(cnf: CNF, v: Variable, c1: Clause, c2: Clause) : (out: bool)
 {
-    exists c1, c2 ::
-        v in cnf_vars(cnf) &&
-        c1 in cnf && c2 in cnf && c1 != c2 &&
-        NotInverted(v) in c1 &&
-        Inverted(v) in c2
+    v in cnf_vars(cnf) &&
+    c1 in cnf && c2 in cnf && c1 != c2 &&
+    NotInverted(v) in c1 &&
+    Inverted(v) in c2
 }
 
-lemma BasicResolution(p: bool, q: bool, r: bool)
-    ensures ((p || q) && (!p || r)) ==> (q || r)
-{
-    
-}
-
-function merge_resolution_specific(v: Variable, vs: map<Variable, bool>, c1: Clause, c2: Clause) : (out: Clause)
+function merge_resolution_specific(v: Variable, ghost vs: map<Variable, bool>, c1: Clause, c2: Clause) : (out: Clause)
     requires v in vs
     requires NotInverted(v) in c1 && Inverted(v) in c2
     ensures (clause_eval(c1, vs) && clause_eval(c2, vs)) ==> clause_eval(out, vs)
@@ -136,146 +73,51 @@ function merge_resolution_specific(v: Variable, vs: map<Variable, bool>, c1: Cla
     c1_others + c2_others
 }
 
-// function merge_resolution(v: Variable, c1: Clause, c2: Clause) : (out: Clause)
-//     requires NotInverted(v) in c1 && Inverted(v) in c2
-//     ensures cnf_equivalent({c1, c2}, {out})
-// {
-//     var orig := {c1, c2};
-
-//     var c1_others := c1 - {NotInverted(v)};
-//     assert forall vs :: v in vs ==> 
-//         clause_eval(c1, vs) == if vs[v] then
-//              true
-//         else
-//             clause_eval(c1_others, vs);
-//     assert forall vs :: v in vs ==> 
-//         clause_eval(c1, vs) == (vs[v] || clause_eval(c1_others, vs));
-
-//     var c2_others := c2 - {Inverted(v)};
-//     assert forall vs :: v in vs ==> 
-//         clause_eval(c2, vs) == if vs[v] then
-//              clause_eval(c2_others, vs)
-//         else
-//             true;
-//     assert forall vs :: v in vs ==> 
-//         clause_eval(c2, vs) == (!vs[v] || clause_eval(c2_others, vs));
-
-//     assert forall vs :: v in vs ==>
-//         BasicResolution(vs[v], clause_eval(c1_others, vs), clause_eval(c2_others, vs));
-//         assert (v[s] || clause_eval(c1_others, vs)) && (!v[s] || clause_eval(c2_others, vs)) == (clause_eval(c1_others, vs) || clause_eval(c2_others, vs));
-
-//     // assert forall vs :: v in vs ==> 
-//     //     if vs[v] then
-//     //         clause_eval(c1, vs) == 
-//     assert forall vs :: v in vs ==> 
-//         if vs[v] then
-//             cnf_eval(orig, vs) == cnf_eval({c2}, vs)
-//         else
-//             cnf_eval(orig, vs) == cnf_eval({c1}, vs);
-
-//     assert forall vs :: v in vs ==> 
-//         if vs[v] then
-//             cnf_eval(orig, vs) == cnf_eval({c2_others}, vs)
-//         else
-//             cnf_eval(orig, vs) == cnf_eval({c1_others}, vs);
-
-//     assert forall vs :: v in vs ==> 
-//         cnf_eval(orig, vs) ==
-//             if vs[v] then
-//                 cnf_eval({c2_others}, vs)
-//             else
-//                 cnf_eval({c1_others}, vs);
-
-//     assert forall vs :: v in vs ==> 
-//         cnf_eval(orig, vs) ==
-//             if vs[v] then
-//                 clause_eval(c2_others, vs)
-//             else
-//                 clause_eval(c1_others, vs);
-    
-//     assert forall vs :: v in vs ==> 
-//         cnf_eval(orig, vs) ==
-//             (clause_eval(c2_others, vs) || clause_eval(c1_others, vs));
-
-//     // assert forall vs :: v in vs ==> 
-//     //     cnf_eval(orig, vs) == (clause_eval(c1, vs) && clause_eval(c2, vs));
-        
-//     // assert forall vs :: v in vs ==> 
-//     //     (   cnf_eval(orig, vs) == cnf_eval({c1_others}, vs) 
-//     //      || cnf_eval(orig, vs) == cnf_eval({c2_others}, vs));
-
-//     // assert forall vs :: v in vs ==> 
-//     //     cnf_eval(orig, vs) == cnf_eval({c1_others + c2_others}, vs);
-
-//     assert forall vs :: v in vs ==>
-//         (clause_eval(c1_others, vs) || clause_eval(c2_others, vs)) == clause_eval(c1_others + c2_others, vs);
-
-
-//     assert forall vs :: v in vs ==> 
-//         cnf_eval(orig, vs) == cnf_eval({c1_others + c2_others}, vs);
-        
-//     var merged := c1_others + c2_others;
-//     merged
-// }
-
-// ghost function cnf_some_resolution_var(cnf: CNF) : (v: Variable)
-//     requires cnf_has_resolution(cnf)
-//     ensures exists l1, l2, c1, c2 ::
-//         c1 in cnf && c2 in cnf && c1 != c2 &&
-//         l1 in c1 && NotInverted(v) == l1 &&
-//         l2 in c2 && Inverted(v) == l2
-// {
-//     assert exists v :: v in cnf_vars(cnf) && cnf_has_resolution_with_var(cnf, v);
-//     var v :| v in cnf_vars(cnf) && cnf_has_resolution_with_var(cnf, v);
-//     v
-// }
-
-// function cnf_clauses_with_var(cnf: CNF, ls: set<ClauseLit>) : (out: set<Clause>)
-//     ensures forall c :: c in cnf && (exists l :: l in ls && l in c) <==> c in out
-// {
-//     set c | c in cnf && (exists l :: l in ls && l in c)
-// }
-
-lemma SetSetWithSomethingInItIsNotEmpty<T>(s: set<T>, f: T -> bool, ss: set<T>)
-    requires exists x :: x in s && f(x)
-    requires ss == set x | x in s && f(x)
-    ensures |ss| > 0
+function merge_resolution(v: Variable, c1: Clause, c2: Clause) : (out: Clause)
+    requires NotInverted(v) in c1 && Inverted(v) in c2
+    ensures cnf_implies({c1, c2}, {out})
+    ensures forall cnf : CNF :: c1 in cnf && c2 in cnf ==> cnf_implies(cnf, cnf - {c1, c2} + {out})
 {
-    var x :| x in s && f(x);
-    assert x in s;
-    assert f(x);
-    assert x in ss;
-    assert |ss| > 0;
+    ghost var example := map[v := true];
+    assert v in example;
+    ghost var vs :| v in vs;
+    merge_resolution_specific(v, vs, c1, c2)
 }
 
-function cnf_resolution(cnf: CNF) : (out: CNF)
-    requires !cnf_has_tautologies(cnf)
-    ensures !cnf_has_resolution(out)
-    ensures cnf_equivalent(cnf, out)
+method cnf_some_resolution(cnf: CNF) returns (v: Variable, c1: Clause, c2: Clause)
+    requires cnf_has_resolution(cnf)
+    ensures cnf_has_resolution_with(cnf, v, c1, c2)
 {
-    // no tautologies
-    assert forall v, l1, l2, c ::
-        v in cnf_vars(cnf) &&
-        c in cnf &&
-        l1 in c && l2 in c ==>
-            l1.invert() != l2;
+    v, c1, c2 :| v in cnf_vars(cnf) && c1 in cnf && c2 in cnf && cnf_has_resolution_with(cnf, v, c1, c2);
+}
 
-    var resolutions: set<(Variable, Clause, Clause)> := set v,c1,c2 
-        | v in cnf_vars(cnf) && c1 in cnf && c2 in cnf && c1 != c2 &&
-            NotInverted(v) in c1 && Inverted(v) in c2
-        :: (v, c1, c2);
-    assert forall r :: r in resolutions ==> (
-        assert r.0 in cnf_vars(cnf);
-        assert exists c1, c2 :: 
-            r.0 in cnf_vars(cnf) &&
-            c1 in cnf && c2 in cnf && c1 != c2
-            && NotInverted(r.0) in c1 && Inverted(r.0) in c2;
+// lemma SetWithSomethingInItIsNotEmpty<T>(s: set<T>, f: T -> bool, ss: set<T>)
+//     requires exists x :: x in s && f(x)
+//     requires ss == set x | x in s && f(x)
+//     ensures |ss| > 0
+// {
+//     var x :| x in s && f(x);
+//     assert x in s;
+//     assert f(x);
+//     assert x in ss;
+//     assert |ss| > 0;
+// }
 
-        cnf_has_resolution_with_var(cnf, r.0)
-        );
-    
+method cnf_resolution_step(cnf: CNF) returns (out: CNF)
+    requires !cnf_has_tautologies(cnf)
+    requires cnf_has_resolution(cnf)
+    ensures cnf_implies(cnf, out)
+    ensures |out| < |cnf|
+{
+    var v,c1,c2 := cnf_some_resolution(cnf);
+    assert NotInverted(v) in c1;
+    assert c1 != c2;
+    var merged := merge_resolution(v, c1, c2);
     assume false;
-    cnf
+
+    assert c1 != merged;
+    assert c2 != merged;
+    out := cnf - {c1, c2} + {merged};
 }
 
 // function cnf_resolution(cnf: CNF) : (out: CNF)
