dfy/util.dfy
@@ -23,6 +23,148 @@ module Util {
         set x, y | y in nested && x in y :: x
     }
 
+    ghost function set_to_seq_spec(s:set<int>) : (out: seq<int>)
+        ensures multiset(s) == multiset(out)
+    {
+        if s == {} 
+        then [] 
+        else 
+            var x := set_pick(s);
+            [x] + set_to_seq_spec(s - {x})
+    }
+
+    method set_to_seq(s:set<int>) returns (out: seq<int>)
+        decreases s
+        ensures multiset(s) == multiset(out)
+        ensures multiset(out) == multiset(set_to_seq_spec(s))
+    {
+        if s == {} {
+            out := [];
+        } else {
+            var x :| x in s;
+            var remaining := set_to_seq(s - {x});
+            out := [x] + remaining;
+        }
+    }
+
+    ghost function set_pick(s: set<int>) : (x: int)
+        requires s != {}
+    {
+        var x :| x in s; x
+    }
+
+    function seq_sum(s: seq<int>) : (sum: int)
+    {
+        if s == [] then
+            0
+        else
+            var x := s[0];
+            var remaining := s[1..];
+            x + seq_sum(remaining)
+    }
+
+    lemma MultiSetAdd(s1: multiset<int>, s2: multiset<int>, add: int)
+        requires s1 + multiset([add]) == s2 + multiset([add])
+        ensures s1 == s2
+    {
+        var added1 := s1 + multiset([add]);
+        var removed1 := added1 - multiset([add]);
+        assert s1 == removed1;
+        var added2 := s2 + multiset([add]);
+        var removed2 := added2 - multiset([add]);
+        assert s2 == removed2;
+    }
+
+    lemma SeqPartsSameSum(s: seq<int>, s1: seq<int>, s2: seq<int>)
+        requires s == s1 + s2
+        ensures seq_sum(s) == seq_sum(s1) + seq_sum(s2)
+    {
+        if s == [] {
+            assert s1 == [];
+            assert s2 == [];
+        } else if s1 == [] {
+            assert s2 == s;
+        } else {
+            var x := s1[0];
+            var s1' := s1[1..];
+            assert s == [x] + s1' + s2;
+            SeqPartsSameSum(s[1..], s1[1..], s2);
+        }
+    }
+
+    lemma DifferentPermutationSameSum(s1: seq<int>, s2: seq<int>)
+        requires multiset(s1) == multiset(s2)
+        ensures seq_sum(s1) == seq_sum(s2)
+    {
+        if s1 == [] {
+            assert s2 == [];
+        } else {
+            var x :| x in s1;
+            assert x in s1;
+            assert multiset(s1)[x] > 0;
+            assert multiset(s2)[x] > 0;
+            assert x in s2;
+            var i1, i2 :| 0 <= i1 < |s1| && 0 <= i2 < |s2| && s1[i1] == s2[i2] && s1[i1] == x;
+
+            var remaining1 := s1[..i1] + s1[i1+1..];
+            assert s1 == s1[..i1] + s1[i1..];
+            assert s1 == s1[..i1] + [x] + s1[i1+1..];
+            assert seq_sum(s1) == seq_sum(s1[..i1] + [x] + s1[i1+1..]);
+            SeqPartsSameSum(s1[..i1+1], s1[..i1], [x]);
+            SeqPartsSameSum(s1, s1[..i1+1], s1[i1+1..]);
+            assert seq_sum(s1) == seq_sum(s1[..i1]) + x + seq_sum(s1[i1+1..]);
+            SeqPartsSameSum(remaining1, s1[..i1], s1[i1+1..]);
+            assert multiset(s1) == multiset(remaining1 + [x]);
+            assert seq_sum(s1) == seq_sum(remaining1) + x;
+            assert multiset(s1) == multiset(remaining1) + multiset([x]);
+            assert multiset(s1) - multiset([x]) == multiset(remaining1);
+
+            var remaining2 := s2[..i2] + s2[i2+1..];
+            assert s2 == s2[..i2] + s2[i2..];
+            assert s2 == s2[..i2] + [x] + s2[i2+1..];
+            assert seq_sum(s2) == seq_sum(s2[..i2] + [x] + s2[i2+1..]);
+            SeqPartsSameSum(s2[..i2+1], s2[..i2], [x]);
+            SeqPartsSameSum(s2, s2[..i2+1], s2[i2+1..]);
+            assert seq_sum(s2) == seq_sum(s2[..i2]) + x + seq_sum(s2[i2+1..]);
+            SeqPartsSameSum(remaining2, s2[..i2], s2[i2+1..]);
+            assert multiset(s2) == multiset(remaining2 + [x]);
+            assert seq_sum(s2) == seq_sum(remaining2) + x;
+            assert multiset(s2) == multiset(remaining2) + multiset([x]);
+            assert multiset(s2) - multiset([x]) == multiset(remaining2);
+
+            DifferentPermutationSameSum(remaining1, remaining2);
+            assert seq_sum(remaining1) == seq_sum(remaining2);
+            assert seq_sum(s1) == seq_sum(s2);
+        }
+    }
+
+    ghost function set_sum_spec(s: set<int>) : (sum: int)
+        ensures seq_sum(set_to_seq_spec(s)) == sum
+    {
+        if s == {} then
+            0
+        else
+            var x := set_pick(s);
+            x + set_sum_spec(s - {x})
+    }
+
+    method set_sum(s: set<int>) returns (sum: int)
+        decreases |s|
+        ensures sum == set_sum_spec(s)
+    {
+        var ss := set_to_seq(s);
+        DifferentPermutationSameSum(ss, set_to_seq_spec(s));
+        sum := seq_sum(ss);
+    }
+
+    lemma SumTests()
+    {
+        assert set_sum_spec({}) == 0;
+        assert set_sum_spec({1}) == 1;
+        assert set_sum_spec({1,2}) == 3;
+        assert set_sum_spec({1,2,3}) == 6;
+    }
+
     function max(a: int, b: int) : (m: int)
         ensures m >= a
         ensures m >= b
